Especificaciones/Envasado/EnvasadoOpt.dfy
@@ -1,23 +1,29 @@
 include "Envasado.dfy"
 
 
-ghost predicate envasarDecissionProblem(A:multiset<nat>, E:nat, k:nat)
+ghost predicate binPackingDecissionProblem(A:multiset<nat>, E:nat, k:nat)
 { 
-  exists I:multiset<multiset<nat>> :: |I| <= k && isEnvasado(A,E,I)   
+  exists I:multiset<multiset<nat>> :: |I| <= k && isBinPacking(A,E,I)   
 }
 
 //POE predicate
-ghost predicate optimalValueEnvasado(A : multiset<nat>, E : nat, k : nat)
-    //requires Envasar(A, E, k)
+ghost predicate optimalValueBinPacking(A : multiset<nat>, E : nat, k : nat)
 {
-    (envasarDecissionProblem(A, E, k)) &&
-    (forall x : nat | x <= |A| && envasarDecissionProblem(A, E, x) :: x >= k)
+    (binPackingDecissionProblem(A, E, k)) &&
+    (forall x : nat | x <= |A| && binPackingDecissionProblem(A, E, x) :: x >= k)
 }
 
-//M to denote multisets
+//I to denote multisets
 //PE predicate
-ghost predicate optimalEnvasado(A : multiset<nat>, E : nat, I:multiset<multiset<nat>>) 
-{      isEnvasado(A, E, I)
-    && forall M : multiset<multiset<nat>> | isEnvasado(A, E, M) :: |M| >= |I|
+ghost predicate optimalBinPacking(A : multiset<nat>, E : nat, I:multiset<multiset<nat>>) 
+{      isBinPacking(A, E, I)
+    && forall M : multiset<multiset<nat>> | isBinPacking(A, E, M) :: |M| >= |I|
+}
+
+//I to denote multisets
+//PE predicate
+ghost predicate optimalBinPackingGeneralization(A : multiset<nat>, E: seq<nat>, I:seq<multiset<nat>>) 
+{      isBinPackingGeneralization(A, E, I)
+    && forall M : seq<multiset<nat>> | isBinPackingGeneralization(A, E, M) :: |M| >= |I|
 }
 
