Especificaciones/Envasado/Envasado.dfy
@@ -7,19 +7,19 @@ include "../Auxiliar/MultisetFacts.dfy"
 // The Bin Packing problem consists of given a multiset of integers A, E y k deciding 
 // if it is possible to divide the multiset elements in a number no larger than k submultisets 
 // such that the sum of elements of each submultiset is no larger than E
-ghost predicate isEnvasado(A : multiset<nat>, E : nat, I:multiset<multiset<nat>>)
+ghost predicate isBinPacking(A : multiset<nat>, E : nat, I:multiset<multiset<nat>>)
 {
        Union(I) == A 
     && forall x | x in I :: x <= A && GSumNat(x) <= E
 }
 
-ghost predicate isEnvasadoSeq(A : multiset<nat>, E : nat, I:seq<multiset<nat>>)
+ghost predicate isBinPackingSeq(A : multiset<nat>, E : nat, I:seq<multiset<nat>>)
 {
        Union(multiset(I)) == A 
     && forall x | x in multiset(I) :: x <= A && GSumNat(x) <= E
 }
 
-ghost predicate isEnvasadoGeneralization(A : multiset<nat>, E: seq<nat>, I:seq<multiset<nat>>)
+ghost predicate isBinPackingGeneralization(A : multiset<nat>, E: seq<nat>, I:seq<multiset<nat>>)
 {
        |I| <= |E|
     && Union(multiset(I[..])) == A 
@@ -27,36 +27,36 @@ ghost predicate isEnvasadoGeneralization(A : multiset<nat>, E: seq<nat>, I:seq<m
 }
 
 // VERIFICACION
-method checkEnvasar(A:multiset<nat>, E:nat, k:nat, I:multiset<multiset<nat>>) returns (b:bool)
+method checkBinPacking(A:multiset<nat>, E:nat, k:nat, I:multiset<multiset<nat>>) returns (b:bool)
 ensures b ==  (|I| <= k 
              && Union(I) == A 
              && forall e | e in I :: (e <= A && GSumNat(e) <= E))
 {
-  var envases := I;
+  var bins := I;
   var b1:= true;
   var union:multiset<nat> := multiset{};
-  while (envases != multiset{} && b1)
-  invariant envases <= I
-  invariant b1 == forall e | e in I - envases :: (e <= A && GSumNat(e) <= E)
-  invariant union == Union(I-envases)
+  while (bins != multiset{} && b1)
+  invariant bins <= I
+  invariant b1 == forall e | e in I - bins :: (e <= A && GSumNat(e) <= E)
+  invariant union == Union(I-bins)
   { 
     
-    ghost var oldenvases := envases;
+    ghost var oldbins := bins;
     ghost var oldunion := union;
-    assert oldunion == Union(I-oldenvases);
+    assert oldunion == Union(I-oldbins);
 
 
-    var e1 := pickMultiset(envases); 
-    envases := envases - multiset{e1};
-    assert I - oldenvases == I-envases-multiset{e1};
+    var e1 := pickMultiset(bins); 
+    bins := bins - multiset{e1};
+    assert I - oldbins == I-bins-multiset{e1};
 
     FSumNatComputaGSumNat(e1);
     b1 := b1 && e1 <= A && FSumNat(e1) <= E;
     
     union := union + e1;
-    UnionOne(I-envases,e1);
+    UnionOne(I-bins,e1);
   }
   assert b1 == forall e | e in I :: (e <= A && GSumNat(e) <= E);
-  assert b1 ==> envases == multiset{} && I-envases == I && union == Union(I);
+  assert b1 ==> bins == multiset{} && I-bins == I && union == Union(I);
   b :=  |I| <= k && b1 && union == A;
 }
