Turing Reducciones/Envasado/PDEToPOE.dfy
@@ -3,13 +3,13 @@ include "../../Especificaciones/Envasado/EnvasadoOpt.dfy"
 
 
 //We assume a polynomial algorithm for POE
-method {:axiom} moptimalEnvasado (A: multiset<nat>, E: nat) returns (I: multiset<multiset<nat>>)
-  ensures optimalEnvasado(A, E, I)
+method {:axiom} moptimalBinPacking(A: multiset<nat>, E: nat) returns (I: multiset<multiset<nat>>)
+  ensures optimalBinPacking(A, E, I)
 
 //We implement a polynomial algorithm for PDE using moptimalEnvasar
 method mEnvasar (A: multiset<nat>, E: nat, k: nat) returns (b:bool)
-  ensures b == envasarDecissionProblem(A, E, k)
+  ensures b == binPackingDecissionProblem(A, E, k)
 {
-  var I := moptimalEnvasado(A, E);
+  var I := moptimalBinPacking(A, E);
   b := |I| <= k;
 }
