Turing Reducciones/Envasado/POEToPOEG.dfy
@@ -1,0 +1,15 @@
+include "../../Especificaciones/Envasado/EnvasadoOpt.dfy"
+
+
+
+//We assume a polynomial algorithm for POEG
+method {:axiom} moptimalBinPackingGeneralization(A: multiset<nat>, E: seq<nat>) returns (I: seq<multiset<nat>>)
+  ensures optimalBinPackingGeneralization(A, E, I)
+
+//We implement a polynomial algorithm for POE using moptimalBinPackingGeneralization
+method moptimalBinPacking(A: multiset<nat>, E: nat, k: nat) returns (I: multiset<multiset<nat>>)
+  ensures optimalBinPacking(A, E, I)
+{
+    //Como sabemos el tamaño de E para hacer la llamada a moptimalBinPackingGeneralization ?
+    assume false;
+}
